src/program_proof/pav/evidence.v
@@ -6,25 +6,143 @@ From Perennial.program_proof Require Import std_proof.
 From iris.unstable.base_logic Require Import mono_list.
 From Perennial.base_logic Require Import ghost_map.
 
+Section other.
+Context `{!heapGS Σ, !pavG Σ}.
+Definition is_link epoch prevLink dig link : iProp Σ :=
+  is_hash (chainSepSome.encodesF (chainSepSome.mk epoch prevLink dig)) link.
+
+Lemma is_link_determ epoch prevLink dig link0 link1 :
+  is_link epoch prevLink dig link0 -∗
+  is_link epoch prevLink dig link1 -∗
+  ⌜ link0 = link1 ⌝.
+Proof.
+  iIntros "Hlink0 Hlink1".
+  by iDestruct (is_hash_deterministic with "Hlink0 Hlink1") as %->.
+Qed.
+
+Lemma is_link_inj epoch0 prevLink0 dig0 epoch1 prevLink1 dig1 link :
+  is_link epoch0 prevLink0 dig0 link -∗
+  is_link epoch1 prevLink1 dig1 link -∗
+  ⌜ epoch0 = epoch1 ∧ prevLink0 = prevLink1 ∧ dig0 = dig1 ⌝.
+Proof.
+  iIntros "Hlink0 Hlink1".
+  iDestruct (is_hash_inj with "Hlink0 Hlink1") as %Heq.
+  by pose proof (chainSepSome.inj _ _ Heq) as [=->].
+Qed.
+End other.
+
 Section evidence.
 Context `{!heapGS Σ, !pavG Σ}.
 
-Definition evidServLink_valid pk evid : iProp Σ :=
+Definition valid_signedLink pk (obj : signedLink.t) link : iProp Σ :=
+  "#His_link" ∷ is_link obj.(signedLink.epoch) obj.(signedLink.prevLink)
+    obj.(signedLink.dig) link ∗
+  "#Hvalid_lnSig" ∷ is_sig pk (servSepLink.encodesF (servSepLink.mk link)) obj.(signedLink.sig).
+
+Definition valid_signedPut pk (obj : signedPut.t) : iProp Σ :=
+  "#Hvalid_putSig" ∷ is_sig
+    pk
+    (servSepPut.encodesF (servSepPut.mk
+      obj.(signedPut.epoch) obj.(signedPut.id) obj.(signedPut.val)))
+    obj.(signedPut.sig).
+
+Definition valid_evidServLink pk (obj : evidServLink.t) : iProp Σ :=
   ∃ link0 link1,
-  is_hash
-    (chainSepSome.encodesF (chainSepSome.mk
-      evid.(evidServLink.epoch0)
-      evid.(evidServLink.prevLink0)
-      evid.(evidServLink.dig0)))
-    link0 ∗
-  is_hash
-    (chainSepSome.encodesF (chainSepSome.mk
-      evid.(evidServLink.epoch1)
-      evid.(evidServLink.prevLink1)
-      evid.(evidServLink.dig1)))
-    link1 ∗
-  is_sig pk (servSepLink.encodesF (servSepLink.mk link0)) evid.(evidServLink.sig0) ∗
-  is_sig pk (servSepLink.encodesF (servSepLink.mk link1)) evid.(evidServLink.sig1).
+  "#Hvalid_sigLn0" ∷ valid_signedLink pk (obj.(evidServLink.sigLn0)) link0 ∗
+  "#Hvalid_sigLn1" ∷ valid_signedLink pk (obj.(evidServLink.sigLn1)) link1 ∗
+  let epoch0 := obj.(evidServLink.sigLn0).(signedLink.epoch) in
+  let epoch1 := obj.(evidServLink.sigLn1).(signedLink.epoch) in
+  let prevLink1 := obj.(evidServLink.sigLn1).(signedLink.prevLink) in
+  "%Hvalid_epoch_links" ∷
+    ⌜ (epoch0 = epoch1 ∧ link0 ≠ link1)
+      ∨
+      (epoch0 = word.sub epoch1 (W64 1) ∧ link0 ≠ prevLink1) ⌝.
+
+Definition valid_evidServPut pk (obj : evidServPut.t) : iProp Σ :=
+  ∃ link,
+  "#Hvalid_sigLn" ∷ valid_signedLink pk (obj.(evidServPut.sigLn)) link ∗
+  "#Hvalid_sigPut" ∷ valid_signedPut pk (obj.(evidServPut.sigPut)) ∗
+  "#Hvalid_merkle" ∷ valid_merkle_proof
+    obj.(evidServPut.proof)
+    obj.(evidServPut.sigPut).(signedPut.id)
+    obj.(evidServPut.val)
+    obj.(evidServPut.sigLn).(signedLink.dig) ∗
+  let epochLn := obj.(evidServPut.sigLn).(signedLink.epoch) in
+  let epochPut := obj.(evidServPut.sigPut).(signedPut.epoch) in
+  "%valid_epochs" ∷ ⌜ epochLn = epochPut ⌝.
+
+Lemma wp_signedLink_check ptr_sigLn sigLn sl_pk pk γ d0 :
+  {{{
+    "HsigLn" ∷ signedLink.own ptr_sigLn sigLn ∗
+    "Hsl_pk" ∷ own_slice_small sl_pk byteT d0 pk ∗
+    "#Hpk" ∷ is_pk pk (serv_sigpred γ)
+  }}}
+  signedLink__check #ptr_sigLn (slice_val sl_pk)
+  {{{
+    sl_link (link : list w8) (err : bool), RET (slice_val sl_link, #err);
+    "HsigLen" ∷ signedLink.own ptr_sigLn sigLn ∗
+    "Hsl_pk" ∷ own_slice_small sl_pk byteT d0 pk ∗
+    "Hsl_link" ∷ own_slice_small sl_link byteT (DfracOwn 1) link ∗
+    (* in no err case, this lets us learn enough about the link
+    to tie down Hvalid_err. *)
+    "#His_link" ∷ is_link sigLn.(signedLink.epoch) sigLn.(signedLink.prevLink)
+      sigLn.(signedLink.dig) link ∗
+    "Hvalid_err" ∷ (valid_signedLink pk sigLn link -∗ ⌜ err = false ⌝) ∗
+    "Hvalid" ∷ if negb err then valid_signedLink pk sigLn link else True
+  }}}.
+Proof. Admitted.
+(*
+  rewrite /evidServLink__check.
+  iIntros (Φ) "H HΦ"; iNamed "H"; iNamed "Hevid".
+
+  (* first link sig. *)
+  wp_loadField.
+  wp_loadField.
+  wp_loadField.
+  wp_apply wp_allocStruct; [val_ty|];
+    iIntros (ptr_linkSep0) "Hptr_linkSep0".
+  iDestruct (struct_fields_split with "Hptr_linkSep0") as "H";
+    iNamed "H"; iClear "tag".
+  iMod (own_slice_small_persist with "Hsl_prevLink0") as "#Hsl_prevLink0".
+  wp_apply (chainSepSome.wp_encode with "[epoch prevLink data Hsl_prevLink0 Hsl_dig0]").
+  {
+    instantiate (1:=chainSepSome.mk _ _ _).
+    rewrite /chainSepSome.own /=.
+    iExists sl_prevLink0, sl_dig0; iFrame "#∗".
+  }
+  iIntros (sl_link0Enc link0Enc) "H"; iNamed "H";
+    iRename "Hobj" into "Hptr_linkSep0";
+    iRename "Hsl_enc" into "Hsl_link0Enc";
+    rename Henc into Henc_link0.
+  wp_apply (wp_Hash with "Hsl_link0Enc");
+    iIntros (sl_link0 link0) "H"; iNamed "H";
+    iRename "Hdata" into "Hsl_link0Enc";
+    iRename "Hhash" into "Hsl_link0";
+    iRename "His_hash" into "His_hash_link0".
+  iMod (own_slice_small_persist with "Hsl_link0") as "#Hsl_link0".
+  wp_apply wp_allocStruct; [val_ty|];
+    iIntros (ptr_enc0) "Hptr_enc0".
+  iDestruct (struct_fields_split with "Hptr_enc0") as "H";
+    iNamed "H"; iClear "tag".
+  wp_apply (servSepLink.wp_encode with "[link]").
+  {
+    instantiate (1:=servSepLink.mk _).
+    rewrite /servSepLink.own /=.
+    iFrame "#∗".
+  }
+  iIntros (sl_enc0 enc0) "H"; iNamed "H";
+    iRename "Hobj" into "Hptr_enc0";
+    iRename "Hsl_enc" into "Hsl_enc0";
+    rename Henc into Henc_enc0.
+  wp_loadField.
+  wp_apply (wp_Verify with "[Hsl_enc0 Hsl_sig0]"); [iFrame "#∗"|];
+    iIntros (?) "H"; iNamed "H";
+    iRename "Hsig" into "Hsl_sig0";
+    iRename "Hmsg" into "Hsl_enc0";
+    iRename "HP" into "Hsigpred0".
+  destruct ok.
+  2: { wp_pures. by iApply "HΦ". }
+*)
 
 Lemma wp_evidServLink_check ptr_evid evid sl_pk pk γ d0 :
   {{{
@@ -35,13 +153,110 @@ Lemma wp_evidServLink_check ptr_evid evid sl_pk pk γ d0 :
   evidServLink__check #ptr_evid (slice_val sl_pk)
   {{{
     (err : bool), RET #err;
+    "Hevid" ∷ evidServLink.own ptr_evid evid ∗
     "Hsl_pk" ∷ own_slice_small sl_pk byteT d0 pk ∗
-    "#Hvalid_sig" ∷ (evidServLink_valid pk evid -∗ ⌜ err = false ⌝) ∗
-    if negb err then False else True
+    "Hvalid_evid" ∷ (valid_evidServLink pk evid -∗ ⌜ err = false ⌝) ∗
+    if negb err then
+      False ∗
+      valid_evidServLink pk evid
+    else True
   }}}.
-Proof. Admitted.
+Proof.
+  rewrite /evidServLink__check.
+  iIntros (Φ) "H HΦ"; iNamed "H"; iNamed "Hevid".
+
+  (* check links. *)
+  wp_loadField.
+  wp_apply (wp_signedLink_check with "[$HsigLn0 $Hsl_pk $Hpk]"). iEval (rewrite /named).
+  iIntros (sl_link0 link0 err0)
+    "(HsigLn0 & Hsl_pk & Hsl_link0 & #His_link0 & Hvalid_err0 & Hvalid0)".
+  wp_if_destruct.
+  { iApply "HΦ". iFrame. iIntros "!>". iNamed 1. iNamed "Hvalid_sigLn0".
+    iDestruct (is_link_determ with "His_link His_link0") as %->.
+    iDestruct ("Hvalid_err0" with "[]") as %[=]. iFrame "#". }
+  iDestruct "Hvalid0" as "#Hvalid0".
+  wp_loadField.
+  wp_apply (wp_signedLink_check with "[$HsigLn1 $Hsl_pk $Hpk]"). iEval (rewrite /named).
+  iIntros (sl_link1 link1 err1)
+    "(HsigLn1 & Hsl_pk & Hsl_link1 & #His_link1 & Hvalid_err1 & Hvalid1)".
+  wp_if_destruct.
+  { (* not sure why i need to frame this here, but not above. *)
+    iApply "HΦ". iFrame "HsigLn0 ∗". iIntros "!>". iNamed 1. iNamed "Hvalid_sigLn1".
+    iDestruct (is_link_determ with "His_link His_link1") as %->.
+    iDestruct ("Hvalid_err1" with "[]") as %[=]. iFrame "#". }
+  iDestruct "Hvalid1" as "#Hvalid1".
+
+  (* check epochs. *)
+  iEval (rewrite /signedLink.own /named) in "HsigLn0".
+  iDestruct "HsigLn0" as (??????) "(Hepoch0 & HprevLink0 & Hsl_prevLink0
+    & Hdig0 & Hsl_dig0 & Hsig0 & Hsl_sig0)".
+  iEval (rewrite /signedLink.own /named) in "HsigLn1".
+  iDestruct "HsigLn1" as (??????) "(Hepoch1 & HprevLink1 & Hsl_prevLink1
+    & Hdig1 & Hsl_dig1 & Hsig1 & Hsl_sig1)".
+  wp_loadField.
+  wp_loadField.
+  wp_loadField.
+  wp_loadField.
+  wp_if_destruct; move: Heqb1 => Heq_epoch.
+  {
+    wp_apply (wp_BytesEqual with "[$Hsl_link0 $Hsl_link1]").
+    iIntros "[Hsl_link0 Hsl_link1]".
+    case_bool_decide as Heq_ln; iApply "HΦ".
+    -
+      iFrame "Hptr_sigLn0 ∗".
+      (* TODO: not sure why iFrame doesn't handle the True here,
+      even tho it does above. *)
+      iSplit; [|done].
+      iNamed 1. iNamed "Hvalid_sigLn0".
+      iDestruct (is_link_determ with "His_link His_link0") as %->.
+      iClear "His_link".
+      (* TODO: bug. this changes goal to False.
+      iNamed "Hvalid_sigLn1". *)
+      iEval (rewrite /valid_signedLink /named) in "Hvalid_sigLn1".
+      iDestruct "Hvalid_sigLn1" as "[His_link _]".
+      iDestruct (is_link_determ with "His_link His_link1") as %->.
+
+      (* main thing: links are equal. *)
+      iPureIntro.
+      destruct Hvalid_epoch_links as [[_ ?] | [Heq _]]; [done|].
+      rewrite Heq_epoch in Heq.
+      assert (∀ (x : w64), x ≠ word.sub x (W64 1)) as ?.
+      { intros ? H%(f_equal (word.sub x)). by ring_simplify in H. }
+      naive_solver.
+    -
+      (* main challenge: ret errNone, derive contra. *)
+      iAssert (valid_evidServLink pk evid) as "Hvalid2".
+      { iFrame "#". naive_solver. }
+      iFrame "Hptr_sigLn0 ∗#".
+      iSplit; [naive_solver|].
+      iClear "Hvalid2 ∗".
+      iEval (rewrite /valid_signedLink /named) in "Hvalid0 Hvalid1".
+      iDestruct "Hvalid0" as "[_ His_sig0]".
+      iDestruct "Hvalid1" as "[_ His_sig1]".
+      iDestruct (is_sig_to_pred with "Hpk His_sig0") as "{His_sig0} HP0".
+      iDestruct (is_sig_to_pred with "Hpk His_sig1") as "{Hpk His_sig1} HP1".
+      iDestruct (get_serv_sigpred_link with "HP0") as "{HP0} HP0".
+      iDestruct (get_serv_sigpred_link with "HP1") as "{HP1} HP1".
+      iEval (rewrite /serv_sigpred_link /named) in "HP0".
+      iDestruct "HP0" as (??? γtrees0 trees0 digs0 links0)
+        "(Hbind & HmonoIdx0 & Htree_views0 & Hdigs0 & Hdigs_links0 & %Hlink_look0)".
+      iDestruct (is_link_inj with "Hbind His_link0") as %(->&->&->).
+      iClear "Hbind His_link0".
+      iEval (rewrite /serv_sigpred_link /named) in "HP1".
+      iDestruct "HP1" as (??? γtrees1 trees1 digs1 links1)
+        "(Hbind & HmonoIdx1 & Htree_views1 & Hdigs1 & Hdigs_links1 & %Hlink_look1)".
+      iDestruct (is_link_inj with "Hbind His_link1") as %(->&->&->).
+      iClear "Hbind His_link1".
+
+      assert (links0 `prefix_of` links1) as Hpref by admit.
+      iPureIntro.
+      rewrite -Heq_epoch in Hlink_look1.
+      pose proof (prefix_lookup_Some _ _ _ _ Hlink_look0 Hpref) as ?.
+      naive_solver.
+      (* TODO: if have two things, turn into prefix of other. *)
+
+
 (*
-  "#Hbind" ∷ is_hash (chainSepSome.encodesF (chainSepSome.mk epoch prevLink dig)) data.(servSepLink.link) ∗
   rewrite /evidServLink__check.
   iIntros (Φ) "H HΦ"; iNamed "H"; iNamed "Hevid".
 
@@ -222,27 +437,6 @@ Proof. Admitted.
 Qed.
 *)
 
-Definition evidServPut_valid pk evid : iProp Σ :=
-  ∃ link,
-  is_hash
-    (chainSepSome.encodesF (chainSepSome.mk
-      evid.(evidServPut.epoch)
-      evid.(evidServPut.prevLink)
-      evid.(evidServPut.dig)))
-    link ∗
-  is_sig pk (servSepLink.encodesF (servSepLink.mk link)) evid.(evidServPut.linkSig) ∗
-  is_sig pk
-    (servSepPut.encodesF (servSepPut.mk
-      evid.(evidServPut.epoch)
-      evid.(evidServPut.id)
-      evid.(evidServPut.val0)))
-    evid.(evidServPut.putSig) ∗
-  valid_merkle_proof
-    evid.(evidServPut.proof)
-    evid.(evidServPut.id)
-    evid.(evidServPut.val1)
-    evid.(evidServPut.dig).
-
 Lemma wp_evidServPut_check ptr_evid evid sl_pk pk γ d0 :
   {{{
     "Hevid" ∷ evidServPut.own ptr_evid evid ∗
@@ -252,7 +446,8 @@ Lemma wp_evidServPut_check ptr_evid evid sl_pk pk γ d0 :
   evidServPut__check #ptr_evid (slice_val sl_pk)
   {{{
     (err : bool), RET #err;
-    "Hvalid_evid" ∷ (evidServPut_valid pk evid -∗ ⌜ err = false ⌝) ∗
+    "Hsl_pk" ∷ own_slice_small sl_pk byteT d0 pk ∗
+    "Hvalid_evid" ∷ (valid_evidServPut pk evid -∗ ⌜ err = false ⌝) ∗
     if negb err then False else True
   }}}.
 Proof. Admitted.
