src/program_proof/pav/invs.v
@@ -12,62 +12,116 @@ Class pavG Σ :=
   }.
 End shared.
 
-Section epochChain.
+Section chain.
 Context `{!heapGS Σ, !pavG Σ}.
 
-Definition chainSepNone_hashes_to h : iProp Σ :=
-  is_hash [(W8 0)] h.
+(* is_link_conn removes the need to think about records or encoding when
+reasoning about links. *)
+Definition is_link_conn epoch prevLink dig link : iProp Σ :=
+  is_hash (chainSepSome.encodesF (chainSepSome.mk epoch prevLink dig)) link.
+
+Lemma is_link_conn_agree_l epoch prevLink dig link0 link1 :
+  is_link_conn epoch prevLink dig link0 -∗
+  is_link_conn epoch prevLink dig link1 -∗
+  ⌜ link0 = link1 ⌝.
+Proof.
+  iIntros "Hlink0 Hlink1".
+  by iDestruct (is_hash_deterministic with "Hlink0 Hlink1") as %->.
+Qed.
+
+Lemma is_link_conn_agree_r epoch0 prevLink0 dig0 epoch1 prevLink1 dig1 link :
+  is_link_conn epoch0 prevLink0 dig0 link -∗
+  is_link_conn epoch1 prevLink1 dig1 link -∗
+  ⌜ epoch0 = epoch1 ∧ prevLink0 = prevLink1 ∧ dig0 = dig1 ⌝.
+Proof.
+  iIntros "Hlink0 Hlink1".
+  iDestruct (is_hash_inj with "Hlink0 Hlink1") as %Heq.
+  by pose proof (chainSepSome.inj _ _ Heq) as [=->].
+Qed.
+
+(* this version zips the data directly to the links,
+by currying the nextLink.
+not sure how hard it is to work with. *)
+Fixpoint alt_binds_aux (nextLink : list w8) (data links : list (list w8)) : iProp Σ :=
+  match data, links with
+  | [], [] => is_hash [(W8 0)] nextLink
+  | d :: data', l :: links' =>
+    is_link_conn (length data') l d nextLink ∗
+    alt_binds_aux l data' links'
+  | _, _ => False
+  end.
+
+Definition alt_binds data links : iProp Σ :=
+  match reverse links with
+  | [] => False
+  | l :: links' => alt_binds_aux l (reverse data) links'
+  end.
+
+(* this version just talks about the latest link.
+it takes more effort to talk about all links,
+but the resulting object might be easier to reason about
+since it's more "local".
+all digs are on one side and a link is on the other side. *)
+Fixpoint is_link_aux (data : list (list w8)) (link : list w8) : iProp Σ :=
+  match data with
+  | [] => is_hash [(W8 0)] link
+  | d :: data' =>
+    ∃ prevLink,
+    is_link_conn (length data') prevLink d link ∗
+    is_link_aux data' prevLink
+  end.
+
+Definition is_link data link := is_link_aux (reverse data) link.
+
+#[global]
+Instance is_link_pers data link : Persistent (is_link data link).
+Proof. Admitted.
+
+Lemma is_link_agree_l data link0 link1 :
+  is_link data link0 -∗ is_link data link1 -∗ ⌜ link0 = link1 ⌝.
+Proof. Admitted.
+
+Fixpoint suffixer {A : Type} (l : list A) : list (list A) :=
+  match l with
+  | [] => [[]]
+  | x :: l' => suffixer l' ++ [l]
+  end.
+
+Definition prefixer {A : Type} (l : list A) := reverse <$> suffixer (reverse l).
+Compute (prefixer [0; 1; 2]).
+
+Lemma prefix_of_prefixer {A : Type} (l1 l2 : list A) :
+  l1 `prefix_of` l2 →
+  prefixer l1 `prefix_of` prefixer l2.
+Proof. Admitted.
 
 Definition binds (data links : list (list w8)) : iProp Σ :=
-  ∃ init,
-  "%Hinit" ∷ ⌜ links !! 0 = Some init ⌝ ∗
-  "#Hinit_hash" ∷ chainSepNone_hashes_to init ∗
-  (* every link except init was formed by the previous link. *)
-  "#Hbinds" ∷ ([∗ list] epoch ↦ d; l ∈ data; (drop 1 links),
-    ∃ prevLink,
-    ⌜ links !! epoch = Some prevLink ⌝ ∗
-    is_hash (chainSepSome.encodesF (chainSepSome.mk epoch prevLink d)) l).
+  ([∗ list] pref;link ∈ (prefixer data);links,
+    is_link pref link).
 
-(* Can't state this thru stdpp Inj bc data, links related thru iProp, not pure func.
-Maybe if we had a pure hash func, things would be diff. *)
-Lemma binds_inj data0 data1 links0 links1 :
-  binds data0 links0 -∗
-  binds data1 links1 -∗
-  ⌜ data0 = data1 ↔ links0 = links1 ⌝.
-Proof. Admitted.
-End epochChain.
+End chain.
 
 Section global_inv.
 Context `{!heapGS Σ, !pavG Σ}.
-(* state is tied together as follows, all from one γ:
-γ →[mono_list]
-γtrees →[ghost_map_auth]
-trees →[is_tree_dig]
-digs →[binds]
-links. *)
 Definition global_inv γ : iProp Σ :=
   ∃ γtrees trees,
   (* γ commits to all the tree γs, including the next tr. *)
   "HmonoTrees" ∷ mono_list_auth_own γ (1/2) γtrees ∗
   "Htree_views" ∷ ([∗ list] γtr; tr ∈ γtrees; trees,
     ghost_map_auth γtr (1/2) tr).
-(*
-Definition global_inv γ : iProp Σ :=
-  ∃ γtrees trees updates digs links,
-  "HmonoTrees" ∷ mono_list_auth_own γ (1/2) γtrees ∗
-  "Htree_views" ∷ ([∗ list] γtr; tr ∈ γtrees; (trees ++ [updates]),
-    ghost_map_auth γtr (1/2) tr) ∗
-  "#Hdigs" ∷ ([∗ list] tr; dig ∈ trees; digs, is_tree_dig tr dig) ∗
-  "#Hdigs_links" ∷ binds digs links.
-*)
 End global_inv.
 
 Section serv_sigpreds.
 Context `{!heapGS Σ, !pavG Σ}.
 
-Definition serv_sigpred_link γ (data : servSepLink.t) : iProp Σ :=
-  ∃ (epoch : w64) (prevLink dig : list w8) γtrees trees digs links,
-  (* TODO: maybe not need prevLink and dig. doesn't show up anywhere. *)
+(* state is tied together as follows, all from one γ:
+γ →[mono_list]
+γtrees →[ghost_map_auth]
+trees →[is_tree_dig]
+digs →[binds]
+links. *)
+Definition serv_sigpred_link_def γ (data : servSepLink.t) (epoch : w64)
+    (prevLink dig : list w8) γtrees trees digs links : iProp Σ :=
   "#Hbind" ∷ is_hash (chainSepSome.encodesF (chainSepSome.mk epoch prevLink dig)) data.(servSepLink.link) ∗
   "#HmonoIdx" ∷ mono_list_lb_own γ γtrees ∗
   "#Htree_views" ∷ ([∗ list] γtr; tr ∈ γtrees; trees,
@@ -75,6 +129,10 @@ Definition serv_sigpred_link γ (data : servSepLink.t) : iProp Σ :=
   "#Hdigs" ∷ ([∗ list] tr; dig ∈ trees; digs, is_tree_dig tr dig) ∗
   "#Hdigs_links" ∷ binds digs links ∗
   "%Hlink_look" ∷ ⌜ links !! (uint.nat epoch) = Some data.(servSepLink.link) ⌝.
+
+Definition serv_sigpred_link γ data : iProp Σ :=
+  ∃ epoch prevLink dig γtrees trees digs links,
+  serv_sigpred_link_def γ data epoch prevLink dig γtrees trees digs links.
 
 Definition serv_sigpred_put γ (data : servSepPut.t) : iProp Σ :=
   ∃ γtr,
@@ -95,4 +153,140 @@ Definition serv_sigpred γ : (list w8 → iProp Σ) :=
       ⌜servSepPut.encodes data dataSepPut⌝ ∗
       serv_sigpred_put γ dataSepPut
     )%I))%I.
+
+Lemma get_serv_sigpred_link γ o :
+  serv_sigpred γ (servSepLink.encodesF o) -∗
+  serv_sigpred_link γ o.
+Proof.
+  iIntros "[_ [[% [%Henc HP]] | [% [%Henc _]]]]"; last first.
+  { by opose proof (servSep_disj _ Henc). }
+  by apply servSepLink.inj in Henc as ->.
+Qed.
+
+Lemma get_serv_sigpred_put γ o :
+  serv_sigpred γ (servSepPut.encodesF o) -∗
+  serv_sigpred_put γ o.
+Proof.
+  iIntros "[_ [[% [%Henc _]] | [% [%Henc HP]]]]".
+  { by opose proof* (servSep_disj Henc). }
+  by apply servSepPut.inj in Henc as ->.
+Qed.
+
+Lemma big_sepL2_lookup_prefix_l `{!BiAffine PROP} {A B : Type}
+    (Φ : A → B → PROP) l1 l2 l1' :
+  l1' `prefix_of` l1 →
+  ([∗ list] x1;x2 ∈ l1;l2, Φ x1 x2) -∗
+  ⌜ ∃ l2', l2' `prefix_of` l2 ∧ length l1' = length l2' ⌝.
+Proof. Admitted.
+
+Lemma big_sepL2_agree_l `{PROP : bi} {A B : Type}
+    (Φ : nat → A → B → PROP) l1 l2 l3 :
+  (∀ k x1 x2 x2', Φ k x1 x2 -∗ Φ k x1 x2' -∗ ⌜ x2 = x2' ⌝) -∗
+  ([∗ list] k↦x1;x2 ∈ l1;l2, Φ k x1 x2) -∗
+  ([∗ list] k↦x1;x2 ∈ l1;l3, Φ k x1 x2) -∗
+  ⌜ l2 = l3 ⌝.
+Proof. Admitted.
+
+(*
+Lemma sep_auth_agree_l γtrees trees0 trees1 :
+  ([∗ list] γtr;tr ∈ γtrees;trees0, ghost_map_auth_pers γtr tr) -∗
+  ([∗ list] γtr;tr ∈ γtrees;trees1, ghost_map_auth_pers γtr tr) -∗
+  ⌜trees0 = trees1⌝.
+Proof.
+  iIntros "Hsep0 Hsep1".
+  unfold_leibniz; setoid_rewrite list_equiv_lookup; fold_leibniz.
+  iDestruct (big_sepL2_length with "Hsep0") as %Hlen0.
+  iDestruct (big_sepL2_length with "Hsep1") as %Hlen1.
+  iIntros (i).
+  destruct (decide (i < length γtrees)) as [Hbound | Hbound].
+  {
+    apply lookup_lt_is_Some in Hbound as [x0 Hlook0].
+    iDestruct (big_sepL2_lookup_1_some with "Hsep0") as %[x1 Hlook1]; [done|].
+    iDestruct (big_sepL2_lookup_1_some with "Hsep1") as %[x2 Hlook2]; [done|].
+    iDestruct (big_sepL2_lookup with "Hsep0") as "Hauth0"; [done..|].
+    iDestruct (big_sepL2_lookup with "Hsep1") as "Hauth1"; [done..|].
+    iDestruct (ghost_map_auth_pers_pers_agree with "Hauth0 Hauth1") as %->.
+    rewrite Hlook1 Hlook2.
+    done.
+  }
+  {
+    assert (trees0 !! i = None) as ->.
+    { apply lookup_ge_None; lia. }
+    assert (trees1 !! i = None) as ->.
+    { apply lookup_ge_None; lia. }
+    done.
+  }
+Qed.
+*)
+
+Lemma big_sepL2_prefix_carry `{PROP : bi} {A B : Type}
+    (Φ : nat → A → B → PROP) l1 l2 l3 l4 :
+  l1 `prefix_of` l3 ∨ l3 `prefix_of` l1 →
+  (∀ k x1 x2 x2', Φ k x1 x2 -∗ Φ k x1 x2' -∗ ⌜ x2 = x2' ⌝) -∗
+  ([∗ list] k↦x1;x2 ∈ l1;l2, Φ k x1 x2) -∗
+  ([∗ list] k↦x1;x2 ∈ l3;l4, Φ k x1 x2) -∗
+  ⌜ l2 `prefix_of` l4 ∨ l4 `prefix_of` l2 ⌝.
+Proof. Admitted.
+(*
+why is this true?
+start:
+l1;l2
+l3;l4
+l1 prefix_of l3.
+
+prefix lookup lemma:
+exists l4',
+l1;l4'
+l4' prefix_of l4.
+
+agreement lemma:
+l2 = l4'.
+
+so l2 prefix_of l4.
+*)
+(*
+  apply exists_common_prefix in Hpref as (γtrees2 & Hpref0 & Hpref1).
+  iDestruct (big_sepL2_lookup_prefix_l with "Hmap_auth0") as %(trees0' & Hpref2 & Hlen0); [exact Hpref0|].
+  iDestruct (big_sepL2_prefix with "Hmap_auth0") as "Hmap_auth0'"; [done..|].
+  iDestruct (big_sepL2_lookup_prefix_l with "Hmap_auth1") as %(trees1' & Hpref3 & Hlen1); [exact Hpref1|].
+  iDestruct (big_sepL2_prefix with "Hmap_auth1") as "Hmap_auth1'"; [done..|].
+  iDestruct (big_sepL2_agree_r with "[] Hmap_auth0' Hmap_auth1'") as %<-.
+  { iIntros "**". by iApply ghost_map_auth_pers_pers_agree. }
+*)
+
+(* extending the prefix_of property of γtrees all the way down to links. *)
+Lemma serv_sigpred_link_def_prefix γ
+    data0 epoch0 prevLink0 dig0 γtrees0 trees0 digs0 links0
+    data1 epoch1 prevLink1 dig1 γtrees1 trees1 digs1 links1 :
+  serv_sigpred_link_def γ data0 epoch0 prevLink0 dig0 γtrees0 trees0 digs0 links0 -∗
+  serv_sigpred_link_def γ data1 epoch1 prevLink1 dig1 γtrees1 trees1 digs1 links1 -∗
+  ⌜ links0 `prefix_of` links1 ∨ links1 `prefix_of` links0 ⌝.
+Proof.
+  iIntros "#HP0 #HP1".
+  iEval (rewrite /serv_sigpred_link_def /named) in "HP0".
+  iDestruct "HP0" as "(_ & Hlb0 & Hmap_auth0 & Hdigs0 & Hbinds0 & _)".
+  iEval (rewrite /serv_sigpred_link_def /named) in "HP1".
+  iDestruct "HP1" as "(_ & Hlb1 & Hmap_auth1 & Hdigs1 & Hbinds1 & _)".
+  iDestruct (mono_list_lb_valid with "Hlb0 Hlb1") as %Hpref0.
+  iClear "Hlb0 Hlb1".
+
+  iDestruct (big_sepL2_prefix_carry with "[] Hmap_auth0 Hmap_auth1") as %Hpref1.
+  { done. }
+  { iIntros "**". by iApply ghost_map_auth_pers_pers_agree. }
+  iClear "Hmap_auth0 Hmap_auth1".
+  iDestruct (big_sepL2_prefix_carry with "[] Hdigs0 Hdigs1") as %Hpref2.
+  { done. }
+  { iIntros "**". by iApply is_tree_dig_agree. }
+  iClear "Hdigs0 Hdigs1".
+  iEval (rewrite /binds) in "Hbinds0 Hbinds1".
+
+  assert (prefixer digs0 `prefix_of` prefixer digs1 ∨
+    prefixer digs1 `prefix_of` prefixer digs0) as Hpref3.
+  { intuition (eauto using prefix_of_prefixer). }
+  iDestruct (big_sepL2_prefix_carry with "[] Hbinds0 Hbinds1") as %Hpref4.
+  { done. }
+  { iIntros "**". by iApply is_link_agree_l. }
+  done.
+Qed.
+
 End serv_sigpreds.
